AccessExt.v
@@ -1,0 +1,211 @@
+From Coq Require Import Arith.Arith.
+
+From Elo Require Import Util.
+From Elo Require Import Array.
+From Elo Require Import Core.
+From Elo Require Import CoreExt.
+From Elo Require Import ValidAddresses.
+From Elo Require Import Access.
+From Elo Require Import NotAccess.
+
+(* ------------------------------------------------------------------------- *)
+(* preservation                                                              *)
+(* ------------------------------------------------------------------------- *)
+
+Local Lemma nacc_subst_preservation : forall m t tx ad x,
+  ~ access m t ad ->
+  ~ access m tx ad ->
+  ~ access m ([x := tx] t) ad.
+Proof.
+  intros * Hnacc ?. generalize dependent tx.
+  induction t; intros; trivial; simpl;
+  try solve [eapply nacc_iff; inv_nacc Hnacc; eauto using not_access];
+  destruct string_eq_dec; trivial.
+  inv_nacc Hnacc. eapply nacc_iff. eauto using not_access.
+Qed.
+
+Local Lemma nacc_mem_add_preservation : forall m t ad vT,
+  ~ access m t (#m) ->
+  ~ access m t ad ->
+  ~ access (m +++ vT) t ad.
+Proof.
+  intros * Hnacc1 Hnacc2 F. induction F; inv_nacc Hnacc2.
+  decompose sum (lt_eq_lt_dec ad' (#m)); subst; simpl_array; inv_nacc Hnacc1.
+  eapply IHF; trivial. eapply nacc_iff. eauto using not_access.
+Qed.
+
+Local Lemma nacc_mem_set_preservation : forall m t ad ad' v T,
+  ~ access m v ad ->
+  ~ access m t ad ->
+  ~ access m[ad' <- (v, T)] t ad.
+Proof.
+  assert (ge_iff_le : forall m n, m >= n <-> n <= m)
+    by (intros; split; destruct n; eauto).
+  assert (forall m ad ad' v,
+    access m[ad' <- v] m[ad' <- v][ad'].tm ad -> ad' < length m). {
+      intros * H. eapply not_ge. rewrite ge_iff_le. intros ?.
+      rewrite (get_set_invalid memory_default) in H; trivial. inversion H.
+  }
+  (* main proof *)
+  intros * ? ? Hacc. remember (m[ad' <- (v, T)]) as m'.
+  induction Hacc; inv_clear Heqm'; eauto using access.
+  match goal with
+  | _ : ~ access _ <{ & ?ad :: _ }> _ |- _ => 
+    decompose sum (nat_eq_dec ad' ad); subst; try (assert (ad < #m) by eauto)
+  end;
+  simpl_array; eauto using access.
+Qed.
+
+(* ------------------------------------------------------------------------- *)
+
+Local Lemma nacc_tstep_none_preservation : forall m t t' ad,
+  ~ access m t ad ->
+  t --[EF_None]--> t' ->
+  ~ access m t' ad.
+Proof.
+  intros * Hnacc. intros. induction_step; inv_nacc Hnacc;
+  try solve [eapply nacc_iff; eauto using not_access].
+  match goal with H : ~ access _ <{ fn _ _ _ }> _ |- _ => inv_nacc H end.
+  eauto using nacc_subst_preservation.
+Qed.
+
+Local Lemma nacc_tstep_alloc_preservation : forall m t t' ad v T,
+  ad < #m ->
+  forall_memory m (valid_addresses m) ->
+  valid_addresses m t ->
+  ~ access m t ad ->
+  t --[EF_Alloc (#m) v T]--> t' ->
+  ~ access (m +++ (v, T)) t' ad.
+Proof.
+  intros * ? ? ? Hnacc ?.
+  induction_step; inversion_vad; inv_nacc Hnacc; eapply nacc_iff;
+  eauto using not_access, nacc_mem_add_preservation, vad_nacc_length.
+  eapply nacc_ad. eauto using not_eq_sym, Nat.lt_neq.
+  simpl_array. eauto using nacc_mem_add_preservation, vad_nacc_length.
+Qed.
+
+Local Lemma nacc_tstep_read_preservation : forall m t t' ad ad',
+  ~ access m t ad ->
+  t --[EF_Read ad' m[ad'].tm]--> t' ->
+  ~ access m t' ad.
+Proof.
+  intros * Hnacc ?. induction_step; inv_nacc Hnacc;
+  try solve [eapply nacc_iff; eauto using not_access].
+  match goal with H : ~ access _ _ _ |- _ => inv_nacc H end.
+Qed.
+
+Local Lemma nacc_tstep_write_preservation : forall m t t' ad ad' v T,
+  ~ access m t ad ->
+  t --[EF_Write ad' v T]--> t' ->
+  ~ access m[ad' <- (v, T)] t' ad.
+Proof.
+  assert (forall m t t' ad ad' v T,
+    ~ access m t ad ->
+    t --[EF_Write ad' v T]--> t' ->
+    ~ access m v ad)
+    by (intros; induction_step; eauto using access).
+  (* main proof *)
+  intros * Hnacc ?. induction_step; inv_nacc Hnacc;
+  eapply nacc_iff; eauto using not_access, nacc_mem_set_preservation.
+Qed.
+
+Local Lemma nacc_tstep_spawn_preservation : forall m t t' block ad,
+  ~ access m t ad ->
+  t --[EF_Spawn block]--> t' ->
+  ~ access m t' ad.
+Proof.
+  intros * Hnacc ?. induction_step; inv_nacc Hnacc;
+  eapply nacc_iff; eauto using not_access.
+Qed.
+
+Local Corollary nacc_mstep_preservation : forall m m' t t' e ad,
+  ad < #m ->
+  forall_memory m (valid_addresses m) ->
+  valid_addresses m t ->
+  ~ access m t ad ->
+  m / t ==[e]==> m' / t' ->
+  ~ access m' t' ad.
+Proof.
+  intros. inversion_mstep;
+  eauto using nacc_tstep_none_preservation,
+    nacc_tstep_alloc_preservation,
+    nacc_tstep_read_preservation,
+    nacc_tstep_write_preservation.
+Qed.
+
+(* ------------------------------------------------------------------------- *)
+
+Local Lemma nacc_thread_default_preservation : forall m ad,
+  ~ access m thread_default ad.
+Proof.
+  intros. eapply nacc_iff. eauto using not_access.
+Qed.
+
+Local Lemma nacc_spawn_block_preservation : forall m t t' block ad,
+  ~ access m t ad ->
+  t --[EF_Spawn block]--> t' ->
+  ~ access m block ad.
+Proof.
+Abort.
+
+Local Lemma nacc_untouched_threads_preservation :
+  forall m m' ths tid tid' t' e ad,
+    forall_threads ths (fun t => ~ access m t ad) ->
+    tid <> tid' ->
+    tid' < #ths ->
+    m / ths[tid] ==[e]==> m' / t' ->
+    ~ access m' ths[tid'] ad.
+Proof.
+Abort.
+
+Corollary nacc_cstep_preservation : forall m m' ths ths' tid e,
+  forall_memory m (~ access m) ->
+  forall_threads ths (~ access m) ->
+  m / ths ~~[tid, e]~~> m' / ths' ->
+  forall_threads ths' (~ access m').
+Proof.
+Abort.
+
+(* ------------------------------------------------------------------------- *)
+
+Local Lemma nacc_tstep_alloc_mem_preservation : forall m t t' v T,
+  ~ access m t ->
+  forall_memory m (~ access m) ->
+  t --[EF_Alloc (#m) v T]--> t' ->
+  forall_memory  (m +++ (v, T)) (~ access (m +++ (v, T))).
+Proof.
+Qed.
+
+Local Lemma nacc_tstep_write_mem_preservation : forall m t t' ad v T,
+  ~ access m t ->
+  forall_memory m (~ access m) ->
+  t --[EF_Write ad v T]--> t' ->
+  forall_memory m[ad <- (v, T)] (~ access m[ad <- (v, T)]).
+Proof.
+Qed.
+
+Local Corollary nacc_mstep_mem_preservation : forall m m' t t' e,
+  ~ access m t ->
+  forall_memory m (~ access m) ->
+  m / t ==[e]==> m' / t' ->
+  forall_memory m' (~ access m').
+Proof.
+Qed.
+
+Local Corollary nacc_cstep_mem_preservation : forall m m' ths ths' tid e,
+  forall_threads ths (~ access m) ->
+  forall_memory m (~ access m) ->
+  m / ths ~~[tid, e]~~> m' / ths' ->
+  forall_memory m' (~ access m').
+Proof.
+Qed.
+
+(* ------------------------------------------------------------------------- *)
+
+Theorem not_access_preservation : forall m m' ths ths' tid e,
+  forall_program m ths (~ access m) ->
+  m / ths ~~[tid, e]~~> m' / ths' ->
+  forall_program m' ths' (~ access m').
+Proof.
+Qed.
+
