NotAccess.v
@@ -1,0 +1,74 @@
+From Elo Require Import Util.
+From Elo Require Import Array.
+From Elo Require Import Core.
+From Elo Require Import Access.
+
+Inductive not_access (m : mem) : tm -> addr -> Prop :=
+  | nacc_unit : forall ad,
+    not_access m <{ unit }> ad
+
+  | nacc_num : forall n ad,
+    not_access m <{ N n }> ad
+
+  | nacc_ad : forall T ad ad',
+    ad <> ad' ->
+    ~ access m m[ad].tm ad' ->
+    not_access m <{ &ad :: T }> ad'
+
+  | nacc_new : forall T t ad,
+    ~ access m t ad ->
+    not_access m <{ new T t }> ad
+
+  | nacc_load : forall t ad,
+    ~ access m t ad ->
+    not_access m <{ *t }> ad
+
+  | nacc_asg : forall t1 t2 ad,
+    ~ access m t1 ad ->
+    ~ access m t2 ad ->
+    not_access m <{ t1 = t2 }> ad
+
+  | nacc_var : forall x ad,
+    not_access m <{ var x }> ad
+
+  | nacc_fun : forall x Tx t ad,
+    ~ access m t ad ->
+    not_access m <{ fn x Tx t }> ad
+
+  | nacc_call : forall t1 t2 ad,
+    ~ access m t1 ad ->
+    ~ access m t2 ad ->
+    not_access m <{ call t1 t2 }> ad
+
+  | nacc_seq : forall t1 t2 ad,
+    ~ access m t1 ad ->
+    ~ access m t2 ad ->
+    not_access m <{ t1; t2 }> ad
+
+  | nacc_spawn : forall t ad,
+    not_access m <{ spawn t }> ad
+  .
+
+Theorem nacc_iff : forall m t ad,
+  ~ access m t ad <-> not_access m t ad.
+Proof.
+  intros. split; intros Hnacc; destruct t;
+  try (eapply nacc_ad
+    || eapply nacc_asg
+    || eapply nacc_call
+    || eapply nacc_seq);
+  eauto using access, not_access;
+  intros ?; subst; try (inv_acc; inv_clear Hnacc); eauto using access.
+  match goal with
+  | Hnacc : ~ access _ <{ & ?ad :: _ }> ?ad' |- _ =>
+    destruct (nat_eq_dec ad ad'); subst
+  end;
+  eauto using access.
+Qed.
+
+(* ------------------------------------------------------------------------- *)
+(* inversion                                                                 *)
+(* ------------------------------------------------------------------------- *)
+
+Ltac inv_nacc Hnacc :=
+  eapply nacc_iff in Hnacc; inversion Hnacc; subst; eauto using access.
